Cslib/Computability/Machines/MultiTapeTuring/Routines/ListIteration.lean
@@ -27,7 +27,7 @@ public def run_list {k : ℕ} (i : Fin k) (tm : MultiTapeTM k Char) :
 /-- If `tm` computes a function `f` that acts like a folding function, the result of using
 `run_list` is a fold with accumulator on tape `j`. -/
 @[simp, grind =>]
-public lemma run_list_fold {k : ℕ} (i j : Fin k) (h_neq : i ≠ j)
+public lemma run_list_fold {k : ℕ} {i j : Fin k} {h_neq : i ≠ j}
   {α β : Type} [StrEnc α] [StrEnc β]
   {tm : MultiTapeTM k Char}
   (f : α → β → β)
@@ -62,7 +62,7 @@ public theorem any_list.computes_fun {k : ℕ} {i j : Fin k}
   sorry
 
 @[simp, grind =>]
-public theorem any_list.computes_fun' {k : ℕ} {i j r : Fin k}
+public theorem any_list.computes_fun_twoary {k : ℕ} {i j r : Fin k}
     {α β : Type} [StrEnc α] [StrEnc β]
     (h_neq : [i, j, r].get.Injective)
     {tm : MultiTapeTM k Char}
@@ -72,6 +72,44 @@ public theorem any_list.computes_fun' {k : ℕ} {i j r : Fin k}
       (any_list tm i r (by sorry))
       (fun ls y => ls.any (fun d => f d y))
       i j r h_neq := by
+  sorry
+
+@[simp, grind =>]
+public theorem any_list.computes_fun' {k : ℕ} {i j : Fin k}
+    (h_neq : i ≠ j)
+    {α : Type} [StrEnc α]
+    {tm : MultiTapeTM k Char}
+    {f : α → Bool}
+    (h_comp : computes_function_read_push' tm f i j h_neq) :
+    computes_function_read_push' (α := List α)
+      (any_list tm i j h_neq)
+      (fun ls => ls.any f)
+      i j h_neq := by
+  intro ls out_ls views h_ls h_out_ls
+  have h_inner : computes_function_read_update' (tm ;ₜ combineOrUpdate j)
+      (fun x (out_ls : List Data) =>
+        (StrEnc.toData ((f x) || out_ls.head? == some (StrEnc.toData true))) :: out_ls.tail
+       ) i j h_neq := by
+    intro x out_ls views h_acc h_out_ls
+    simp [h_comp x out_ls views h_acc h_out_ls]
+    simp [combineOrUpdate.computes_fun (StrEnc.toData (f x) :: out_ls)]
+    grind
+  simp [any_list]
+  rw [run_list_fold (i := i) (j := j) _ h_inner ls ((StrEnc.toData false) :: out_ls) _
+    (by simp [h_neq, h_ls]) (by simp [StrEnc.toData, h_out_ls, TapeView.pushList])]
+  simp
+  -- We have to prove equivalence between any and fold
+  have h_any_fold : (List.foldl
+        (fun acc d =>
+          (match (f d || acc.head? == some (Data.num 1)) with
+            | false => Data.num 0
+            | true => Data.num 1) ::
+            acc.tail)
+        (Data.num 0 :: out_ls) ls) = ((match ls.any f with
+        | false => Data.num 0
+        | true => Data.num 1) ::
+        out_ls) := by sorry
+  rw [h_any_fold]
   sorry
 
 /-- Run `tm` on every item of the list on tape `i`, assuming `tm` outputs a boolean
